\documentclass{acm_proc_article-sp}

\PassOptionsToPackage{utf8x}{inputenc}

\bibliographystyle{plain}

%agda literal file
\usepackage{agda}

\usepackage{dsfont}
%\let\proof\relax
%\let\endproof\relax
%\usepackage{amsthm}
\usepackage{relsize}
\usepackage{color}
\usepackage{amsmath}
\usepackage{amsfonts}
\usepackage{amssymb}
\usepackage{autofe}
\usepackage{stmaryrd}
\usepackage{textgreek}
\usepackage{ucs}
\usepackage[utf8x]{inputenc}
\usepackage{diagxy}

\usepackage{mypack}

\newcommand{\wig}{weak $\infty$-groupoids}
\newcommand{\og}{$\omega$-groupoids}
\newcommand{\wog}{weak $\omega$-groupoids}
\newcommand{\wogs}{weak $\omega$-groupoid} % s for singular
\newcommand{\hott}{Homotopy Type Theory}
\newcommand{\ott}{Observational Type Theory}
\newcommand{\tig}{$\mathcal{T}_{\infty-groupoid}$}


\newcommand{\new}{\textcolor{red}}

%\let\oldcode\code
%\def\code{\oldcode\tiny}

\begin{document}
\pagenumbering{gobble}
\title{Some constructions on {\huge$\omega$}-groupoids}

\numberofauthors{3}
\author{
% 1st. author
\alignauthor
Thorsten Altenkirch\\
       \affaddr{University of Nottingham}\\
       \affaddr{United Kingdom}\\
       \email{txa@cs.nott.ac.uk}
% 2nd. author
\alignauthor
Nuo Li\\
       \affaddr{University of Nottingham}\\
       \affaddr{United Kingdom}\\
       \email{nzl@cs.nott.ac.uk}
% 3rd. author
\alignauthor
Ond\v{r}ej Ryp\'a\v{c}ek\\
       \affaddr{University of Oxford}\\
       \affaddr{United Kingdom}\\
       \email{ondrej.rypacek@gmail.com}
}


\newcommand{\txa}[1]{\marginpar{txa:#1}}
\newcommand{\oxr}[1]{\marginpar{\footnotesize oxr:#1}}

\maketitle


\AgdaHide{
\begin{code}%
\>\AgdaSymbol{\{-\#} \AgdaKeyword{OPTIONS} --type-in-type --no-positivity-check --no-termination-check \AgdaSymbol{\#-\}}\<%
\\
%
\\
%
\\
\>\AgdaKeyword{module} \AgdaModule{BasicSyntax} \AgdaKeyword{where} \<[25]%
\>[25]\<%
\\
%
\\
%
\\
\>\AgdaKeyword{open} \AgdaKeyword{import} \AgdaModule{Relation.Binary.PropositionalEquality}\<%
\\
\>\AgdaKeyword{open} \AgdaKeyword{import} \AgdaModule{Function}\<%
\\
\>\AgdaKeyword{open} \AgdaKeyword{import} \AgdaModule{Data.Product} \AgdaKeyword{renaming} \AgdaSymbol{(}\_,\_ \AgdaSymbol{to} \_,,\_\AgdaSymbol{)}\<%
\\
%
\\
%
\\
\>\AgdaKeyword{infix} \AgdaNumber{4} \_≅\_\<%
\\
\>\AgdaKeyword{infix} \AgdaNumber{4} \_=h\_\<%
\\
\>\AgdaKeyword{infixl} \AgdaNumber{6} \_+T\_ \_+S\_ \_+tm\_\<%
\\
\>\AgdaKeyword{infixl} \AgdaNumber{5} \_,\_\<%
\\
\>\AgdaKeyword{infixl} \AgdaNumber{7} \_⊚\_\<%
\\
%
\\
\>\<%
\end{code}
}

\begin{abstract}

  Weak $\omega$-groupoids are the higher dimensional generalisation of
  setoids and are an essential ingredient of the constructive
  semantics of Homotopy Type Theory \cite{hott}.  Following up on our previous formalisation \cite{txa:csl}
  and Brunerie's notes \cite{gb:wog}, we present a new formalisation of the syntax
  of weak $\omega$-groupoids in Agda using heterogeneous equality. We show how 
  to recover basic constructions on $\omega$-groupoids using suspension and replacement. In particular we show that any type forms 
  a groupoid and that we can derive higher dimensional composition. We present a possible semantics using globular sets and discuss
  the issues which arise when using globular types instead.

% In \hott{}, a variant of \mltt{}, we reject proof-irrelevance so that the common interpretation of types as setoids has to be generalised. With the univalence axiom, we treat equivalence as equality and interpret types as \og{}. Inspired by Altenkirch's work \cite{txa:csl} and Brunerie's notes \cite{gb:wog}, we study and implement a syntactic definition of Grothendieck \wog{} in Agda which is a popular variant of \mltt{} and a famous theorem prover. It is the first step to model type theory with \wog{} so that we could eliminate the univalence axiom.

\end{abstract}

\category{F.4.1}{Mathematical Logic and Formal Languages}{Lambda calculus and related systems, Mechanical theorem proving}

\terms{Theory}

\keywords{Type Theory, Homotopy Type Theory, Category Theory, Higher dimensional structures, \new{Agda}}



\section{Introduction}

% Background

%why do we need to use omega groupoid

In Type Theory, a type can be interpreted as a setoid which is a set equipped with an equivalence relation \cite{alti:lics99}.
The equivalence proof of the relation consists of reflexivity, symmetry and transitivity whose proofs are unique. 
However in \hott{}, we reject the principle of uniqueness of identity proofs (UIP). 
Instead we accept the univalence axiom which says that equality of types is weakly equivalent to weak equivalence. 
Weak equivalence can be seen as a refinement of isomorphism without UIP \cite{txa:csl}. 
For example, a weak equivalence 
between two objects A and B in a 2-category is a morphism $f : A \rightarrow B$ which has a
corresponding inverse morphism $ g : B \rightarrow A$, but instead of the
proofs of isomorphism $f ∘ g = 1_B$ and  $g ∘ f = 1_A$ we have two
2-cell isomorphisms  $f ∘ g ≅ 1_B$ and  $g ∘ f ≅ 1_A$. 

Voevodsky proposed the univalence axiom which basically says that
isomorphic types are equal. This can be viewed as a strong
extensionality axiom and it does imply functional extensionality.
%(a coq proof of this can be found in \cite{uafe})
However, adding
univalence as an axiom destroys canonicity, i.e. that every closed
term of type $\mathbb{N}$ is reducible to a numeral. In the special case of
extensionality and assuming a strong version of UIP we were able to
eliminate this issue \cite{alti:lics99,alti:ott-conf} using
setoids. However, it is not clear how to generalize this in the
absence of UIP to
univalence which is incompatible with UIP.  To solve the problem we
should generalise the notion of setoids, namely to enrich the
structure of the identity proofs.


The generalised notion is called {\wog} and was proposed by
Grothendieck 1983 in a famous manuscript \emph{Pursuing Stacks} \cite{gro:ps}. Maltsiniotis continued his work and suggested a simplification of the original definition which can be found in \cite{mal:gwog}. Later Ara also presents a slight variation of the simplication of {\wog} in \cite{ara:wog}. Categorically speaking an $\omega$-groupoid is an $\omega$-category in which morphisms on all levels are equivalences. As we know that a set can be seen as a discrete
category, a setoid is a category where every morphism is unique between
two objects. A groupoid is more generalised, every morphism is
isomorphism but the proof of isomorphism is unique, namely the composition of a morphism with its inverse is equal to an identity morphism. Similarly, an
n-groupoid is an n-category in which morphisms on all levels are
equivalence. {\og} which are also called $\infty$-groupoids is an
infinite version of n-groupoids. To model Type Theory without UIP we
also require the equalities to be non-strict, in other words, they are
not definitionally equalities. Finally we should use {\wog} to interpret types and eliminate the univalence axiom.

There are several approaches to formalise {\wog} in Type Theory. For instance, Altenkirch and Ryp\'a\v{c}ek \cite{txa:csl}, and Brunerie's notes \cite{gb:wog}.
This paper explains an implementation of {\wog} following Brunerie's approach in Agda which is a well-known theorem prover and also a variant of intensional {\mltt}. This is the first attempt to formalise this approach in a dependently typed language like Agda or Coq. The approach is to specify when a globular set is a {\wogs} by first defining a type theory called {\tig} to describe the internal language
of Grothendieck {\wog}, then interpret it with a globular set and a dependent function. All coherence laws of the {\wog} are derivable from the syntax, we will present some basic ones, for example reflexivity. One of the main contributions of this paper is to use heterogeneous equality for terms to overcome some difficult problems we encountering when using the normal homogeneous one. In this paper, we omit some complicated and less important programs, namely the proofs of some lemmas or definitions of some auxiliary functions. It is still possible for the reader who is interested in the details to check the code online \footnote{The code is available on }, in which there are only some minor differences.

\subsection*{Agda}

Agda is a programming language and development environment based on
Martin-Löf Type Theory \cite{agda-wiki}. Readers with background in
Type Theory (e.g. from reading the introductory chapters of
\cite{hott}) should find it easy to read the Agda code presented
in this paper. Some hints: $\Pi$-types are written in a generalized
arrow notation $(x : A) → B$ for $\Pi x:A.B$, implicit arguments are
indicated by curly brackets, eg. $\{x : A\} → B$, in this case the Agda
will try to generate the argument automatically and we don't supply it
to make the code more readable. If we don't want to supply $A$ because
it can be inferred we write $\forall x$ or $\forall\{x\}$.
Agda uses a flexible mixfix notation
where the position of arguments are indicated by underline characters.
e.g. $\_⇒\_$ is one identifier which can be applied to two arguments as
in $A ⇒ B$.  
We use data \textbf{data} to define constructor based datatypes (both
inductive and coinductive) and \textbf{record} to define dependent record
types (this generalizes $\Sigma$-types. The representation of
coinductive types and more generally mixed inductive/coinductive types
\cite{txa:mpc2010g}
uses the type constructor $\infty$ whose elements are computations of type
$A$ which are written as $\sharp a$ where |a| is an expression which can be
evaluated to an element of type $A$.

\section*{Acknowledgements}

The first and second author would like to thank the organizers and
other participants of the special year on homotopy type theory at the
Institute for Advanced Study where they had many interesting
discussion topics related to the work presented in this
paper. Especially we all would like to acknowledge Guillaume
Brunerie's proposal which made this work possible. 




\section{Syntax}\label{sec:syntax}

We develop the type theory of $\omega$-groupoids formally, following
\cite{gb:wog}. This is a Type Theory with only one type former which
we can view as equality types and interpret as the homsets of the
$\omega$-groupoid. There are no definitional equalities which
correspond to the fact that we consider weak $\omega$-groupoids. None of the groupoid laws on any levels are strict (i.e. definitional) but all are witnessed by
terms. Compared to \cite{txa:csl} the definition is very much
simplified by the observation that all laws of a weak $\omega$-groupoid follow from the existence of coherence constants for
any contractible context.

In our formalisation we exploit the more liberal way to do mutual
definitions in Agda, which was implemented recently following up a
suggestion by the first author. It allows us to first introduce a type
former but give its definition later.

Since we are avoiding definitional equalities we have to define a
syntactic substitution operation which we need for the general
statement of the coherence constants. However, defining this constant
requires us to prove a number of substitution laws at the same
time. We address this issue by using a heterogeneous equality which
exploits UIP. Note that UIP holds for
the syntax because all components defined here
are sets in the sense of Homotopy Type Theory.

% Since the definitions of contexts, types and terms involve each others, we adopt a more liberal way to do mutual definition in Agda which is a feature available since version 2.2.10. Something declared is free to use even it has not been completely defined.


\subsection{Basic Objects}

We first declare the syntax of our type theory which is
called \tig{} namely the internal language of \wog. Since the definitions of syntactic objects involve each others, it is essential to define them in a inductive-inductive way. Agda allows us to state the types and constructors separately for involved inductive-inductive definitions. The following declarations in order are contexts as sets,
types are sets dependent on contexts, terms and variables are sets
dependent on types, Contexts morphisms and the contractible contexts.

\begin{code}%
\>\AgdaKeyword{
dat}a\AgdaDatatype{ Co}n           :\AgdaPrimitiveType{ Se}t\AgdaKeyword{
dat}a\AgdaDatatype{ T}y \AgdaBound{(}Γ :\AgdaDatatype{ Co}\AgdaSymbol{n})  :\AgdaPrimitiveType{ Se}t\AgdaKeyword{
dat}a\AgdaDatatype{ T}m            : \AgdaBound{\{}Γ :\AgdaDatatype{ Co}\AgdaSymbol{n\}}\AgdaBound{(}A :\AgdaDatatype{ T}y \AgdaSymbol{Γ}) →\AgdaPrimitiveType{ Se}t\AgdaKeyword{
dat}a\AgdaDatatype{ Va}r           : \AgdaBound{\{}Γ :\AgdaDatatype{ Co}\AgdaSymbol{n\}}\AgdaBound{(}A :\AgdaDatatype{ T}y \AgdaSymbol{Γ}) →\AgdaPrimitiveType{ Se}t\AgdaKeyword{
dat}a\AgdaDatatype{ \_⇒}\_           :\AgdaDatatype{ Co}n →\AgdaDatatype{ Co}n →\AgdaPrimitiveType{ Se}t\AgdaKeyword{
dat}a\AgdaDatatype{ isCont}r       :\AgdaDatatype{ Co}n →\AgdaPrimitiveType{ Se}t
\<%
\end{code}
Contexts are inductively defined as either an empty context or
a context with a type in it.

\begin{code}%
\>\AgdaKeyword{
dat}a\AgdaDatatype{ Co}n\AgdaKeyword{ wher}e
  ε     :\AgdaDatatype{ Co}n
 \AgdaInductiveConstructor{ \_,}\_   : \AgdaBound{(}Γ :\AgdaDatatype{ Co}\AgdaSymbol{n)}\AgdaBound{(}A :\AgdaDatatype{ T}y \AgdaSymbol{Γ}) →\AgdaDatatype{ Co}n
\<%
\end{code}
Types are defined as either $*$ which we
call 0-cells, or a equality type between two terms of some type A. If 
type A is n-cell then we call its equality type $(n+1)$-cell.

\begin{code}%
\>\AgdaKeyword{
dat}a\AgdaDatatype{ T}y Γ\AgdaKeyword{ wher}e
  *     :\AgdaDatatype{ T}y Γ
 \AgdaInductiveConstructor{ \_=h}\_  : \AgdaBound{\{}A :\AgdaDatatype{ T}y \AgdaSymbol{Γ\}}\AgdaBound{(}a b :\AgdaDatatype{ T}m \AgdaSymbol{A}) →\AgdaDatatype{ T}y Γ
\<%
\end{code}

\subsection{Heterogeneous Equality for Terms}

One of the big challenges we encountered at first is the difficulty to
formalise and to reason about the equalities of terms, which is
essential when defining substitution.  When the usual identity types
are used which are homogeneous, one has to use substitution to unify
the types on both sides of equality types. This results in
$\mathit{subst}$ to appear in terms, about which one has to state
substitution lemmas. This further pollutes syntax requiring lemmas
about lemmas, lemmas about lemmas about lemmas, etc. \new{For example, we have to prove using $\mathit{subst}$ consecutively with two equalities of types is propositionally equal to using $\mathit{subst}$ with the composition of these two equalities. There are more and more lemmas needed as the complexity of the proofs grows.} The resulting
recurrence pattern has been identified and implemented in
\cite{txa:csl} for the special cases of coherence cells for
associativity, units and interchange. However it is not clear how that
approach could be adapted to the present, much more economical
formulation of {\wog}. Moreover, the complexity brings the
Agda type checker to its limits and correctness into question.

The idea of heterogenous equality, which we use to resolve this issue,
is that one can define equality for terms of different types, but its
inhabitants only for terms of definitionally equal types. However, the
corresponding elimination principle relies on UIP. \new{In intensional type theory, UIP is not provable in general,
  namely not all types are h-sets (homotopy 0-types). However it is
  justified to claim all type with decidable equality are h-sets.
  From the Hedberg's Theorem \cite{hed:98} we know that inductive
  types with finitary constructors have decidable equality. In our
  case, the types which stand for syntactic objects (contexts, types, terms)
  are all inductive-inductive types with finitary constructors and it is
  therefore safe to assume UIP holds for them. }
In summary, the equality of
syntactic types is unique, so it is safe to use heterogeneous equality
and do without the substitution lemmas which would otherwise be
necessary to match terms of different types. \new{From a computational perspective, it means that every equality of types can be reduced to $\mathit{refl}$ and using $\mathit{subst}$ to construct terms is proof-irrelevant, which is expressed in the definition of heterogeneous equality for terms. }


\begin{code}%
\>\AgdaKeyword{
dat}a\AgdaDatatype{ \_≅}\_ \AgdaBound{\{}Γ :\AgdaDatatype{ Co}\AgdaSymbol{n\}}\AgdaBound{\{}A :\AgdaDatatype{ T}y \AgdaSymbol{Γ}\} :
         \AgdaBound{\{}B :\AgdaDatatype{ T}y \AgdaSymbol{Γ}\} →\AgdaDatatype{ T}m A →\AgdaDatatype{ T}m B →\AgdaPrimitiveType{ Se}t\AgdaKeyword{ wher}e
 \AgdaInductiveConstructor{ ref}l : \AgdaBound{(}b :\AgdaDatatype{ T}m \AgdaSymbol{A}) → b ≅ b
\<%
\end{code}


\AgdaHide{
\begin{code}%
\>\AgdaFunction{
\_-}¹          :\AgdaSymbol{ ∀}\AgdaBound{\{}Γ :\AgdaDatatype{ Co}\AgdaSymbol{n\}}\AgdaBound{\{}A B :\AgdaDatatype{ T}y \AgdaSymbol{Γ\}}\AgdaBound{\{}a :\AgdaDatatype{ T}m \AgdaSymbol{A\}}\AgdaBound{\{}b :\AgdaDatatype{ T}m \AgdaSymbol{B}\} → a ≅ b → b ≅ a\<%
\\
\>\AgdaInductiveConstructor{(ref}l\AgdaSymbol{ \_})\AgdaFunction{ -}¹  =\AgdaInductiveConstructor{ ref}l \_
\AgdaKeyword{
infix}r 4 \_∾\_ 
\AgdaFunction{
\_∾}\_ : \AgdaBound{\{}Γ :\AgdaDatatype{ Co}\AgdaSymbol{n}\}
      \AgdaBound{\{}A B C :\AgdaDatatype{ T}y \AgdaSymbol{Γ}\}
      \AgdaBound{\{}a :\AgdaDatatype{ T}m \AgdaSymbol{A\}}\AgdaBound{\{}b :\AgdaDatatype{ T}m \AgdaSymbol{B\}}\AgdaBound{\{}c :\AgdaDatatype{ T}m \AgdaSymbol{C}\} →
      a ≅ b → 
      b ≅ c 
    → a ≅ c\AgdaFunction{
\_∾}\_ \{c = \AgdaSymbol{c}\} \AgdaInductiveConstructor{(ref}l \AgdaBound{.}\AgdaSymbol{c}) \AgdaInductiveConstructor{(ref}l \AgdaBound{.}\AgdaSymbol{c}) =\AgdaInductiveConstructor{ ref}l c


\<%
\end{code}
}
Once we have the heterogeneous equality for terms, we can define a proof-irrelevant substitution which we call coercion here
since it gives us a term of type A if we have a term of type B and the
two types are equal. We can also prove that the coerced term is heterogeneously equal to the
original term. Combining these definitions, it is much
more convenient to formalise and to reason about term equations.

\begin{code}%
\>\AgdaFunction{
\_⟦\_}⟫        : \AgdaBound{\{}Γ :\AgdaDatatype{ Co}\AgdaSymbol{n\}}\AgdaBound{\{}A B :\AgdaDatatype{ T}y \AgdaSymbol{Γ\}}\AgdaBound{(}a :\AgdaDatatype{ T}m \AgdaSymbol{B}) 
            → A ≡ B →\AgdaDatatype{ T}m A\<%
\\
\>a ⟦\AgdaInductiveConstructor{ ref}l ⟫  = a
\AgdaFunction{
cohO}p       : \AgdaBound{\{}Γ :\AgdaDatatype{ Co}\AgdaSymbol{n\}}\AgdaBound{\{}A B :\AgdaDatatype{ T}y \AgdaSymbol{Γ\}}\AgdaBound{\{}a :\AgdaDatatype{ T}m \AgdaSymbol{B\}}\AgdaBound{(}p : A ≡ \AgdaSymbol{B}) 
            → a ⟦ p ⟫ ≅ a\AgdaFunction{
cohO}p\AgdaInductiveConstructor{ ref}l  =\AgdaInductiveConstructor{ ref}l \_
\<%
\end{code}

% could delete the explanation of this lemma

%It is sufficient to prove the original terms are equal if we coerced them using the same proof. This lemma is useful later.

\AgdaHide{
\begin{code}%
\>\AgdaFunction{
cohOp-e}q : \AgdaBound{\{}Γ :\AgdaDatatype{ Co}\AgdaSymbol{n\}}\AgdaBound{\{}A B :\AgdaDatatype{ T}y \AgdaSymbol{Γ\}}\AgdaBound{\{}a b :\AgdaDatatype{ T}m \AgdaSymbol{B\}}\AgdaBound{\{}p : A ≡ \AgdaSymbol{B}\} → \AgdaBound{(}a ≅ \AgdaSymbol{b}) 
         → \AgdaBound{(}a ⟦ p ⟫ ≅ b ⟦ p \AgdaSymbol{⟫})\AgdaFunction{
cohOp-e}q \AgdaBound{\{}\AgdaSymbol{Γ}\} \AgdaSymbol{\{}\AgdaBound{.}\AgdaSymbol{B}\} \AgdaBound{\{}\AgdaSymbol{B}\} \AgdaBound{\{}\AgdaSymbol{a}\} \AgdaBound{\{}\AgdaSymbol{b}\} \AgdaInductiveConstructor{\{ref}\AgdaSymbol{l}\} r = r
\AgdaFunction{
cohOp-ho}m : \AgdaBound{\{}Γ :\AgdaDatatype{ Co}\AgdaSymbol{n\}}\AgdaBound{\{}A B :\AgdaDatatype{ T}y \AgdaSymbol{Γ\}}\AgdaBound{\{}a b :\AgdaDatatype{ T}m \AgdaSymbol{B\}}\AgdaBound{(}p : A ≡ \AgdaSymbol{B}) → \AgdaBound{(}a ⟦ p ⟫\AgdaInductiveConstructor{ =}h b ⟦ p \AgdaSymbol{⟫}) ≡ \AgdaBound{(}a\AgdaInductiveConstructor{ =}h \AgdaSymbol{b})\AgdaFunction{
cohOp-ho}m\AgdaInductiveConstructor{ ref}l =\AgdaInductiveConstructor{ ref}l
\AgdaFunction{
cong}≅ : \AgdaBound{\{}Γ Δ :\AgdaDatatype{ Co}\AgdaSymbol{n\}}\AgdaBound{\{}A B :\AgdaDatatype{ T}y \AgdaSymbol{Γ\}}\AgdaBound{\{}a :\AgdaDatatype{ T}m \AgdaSymbol{A\}}\AgdaBound{\{}b :\AgdaDatatype{ T}m \AgdaSymbol{B\}}\AgdaBound{\{}D :\AgdaDatatype{ T}y Γ →\AgdaDatatype{ T}y \AgdaSymbol{Δ}\} →
        \AgdaBound{(}f : \AgdaBound{\{}C :\AgdaDatatype{ T}y \AgdaSymbol{Γ}\} →\AgdaDatatype{ T}m C →\AgdaDatatype{ T}m \AgdaBound{(}D \AgdaSymbol{C)}) → 
        a ≅ b 
      → f a ≅ f b\AgdaFunction{
cong}≅ f \AgdaInductiveConstructor{(ref}l\AgdaSymbol{ \_}) =\AgdaInductiveConstructor{ ref}l \_

\<%
\end{code}
}


\subsection{Substitutions}

With context morphisms, we can define substitutions for types
variables and terms.  Usually we define a set of symbols together and
we name a function $*$ as $*C$ for contexts, $*T$ for types, $*V$ for
variables $*tm$ for terms and $*S$ (or $*cm$) for context morphisms. For example
the substitution for types is defined as follows

\begin{code}%
\>\AgdaFunction{
\_[\_]}T   :\AgdaSymbol{ ∀}\AgdaBound{\{}Γ \AgdaSymbol{Δ}\} →\AgdaDatatype{ T}y Δ → Γ ⇒ Δ →\AgdaDatatype{ T}y Γ\AgdaFunction{
\_[\_]}V   :\AgdaSymbol{ ∀}\AgdaBound{\{}Γ Δ \AgdaSymbol{A}\} →\AgdaDatatype{ Va}r A → \AgdaBound{(}δ : Γ ⇒ \AgdaSymbol{Δ}) →\AgdaDatatype{ T}m \AgdaBound{(}A [ δ\AgdaFunction{ ]}\AgdaSymbol{T})\AgdaFunction{
\_[\_]t}m  :\AgdaSymbol{ ∀}\AgdaBound{\{}Γ Δ \AgdaSymbol{A}\} →\AgdaDatatype{ T}m A → \AgdaBound{(}δ : Γ ⇒ \AgdaSymbol{Δ}) →\AgdaDatatype{ T}m \AgdaBound{(}A [ δ\AgdaFunction{ ]}\AgdaSymbol{T})    
\<%
\end{code}
Indeed the
composition of contexts can be understood as substitution for context morphisms as well.

\begin{code}%
\>\AgdaFunction{
\_⊚}\_ :\AgdaSymbol{ ∀}\AgdaBound{\{}Γ Δ \AgdaSymbol{Θ}\} → Δ ⇒ Θ → \AgdaBound{(}δ : Γ ⇒ \AgdaSymbol{Δ}) → Γ ⇒ Θ   
\<%
\end{code}

\AgdaHide{
\begin{code}%
\>\AgdaComment{
-- \_[\_]T   : \{Γ Δ : Con\}            → Ty Δ    → (δ : Γ ⇒ Δ)   → Ty Γ       } \AgdaComment{
-- \_[\_]V   : \{Γ Δ : Con\}\{A : Ty Δ\}  → Var A   → (δ : Γ ⇒ Δ)   → Tm (A [ δ ]T})\AgdaComment{
-- \_[\_]tm  : \{Γ Δ : Con\}\{A : Ty Δ\}  → Tm A    → (δ : Γ ⇒ Δ)   → Tm (A [ δ ]T)   } \AgdaComment{
-- \_⊚\_     : \{Γ Δ Θ : Con\}          → Δ ⇒ Θ → (δ : Γ ⇒ Δ)   → Γ ⇒ Θ  } \<%
\end{code}
}


\subsection{Weakening Rules}

We can freely add types to the contexts of any given type judgments,
term judgments or context morphisms. These are weakening rules.

\begin{code}%
\>\AgdaFunction{
\_+T}\_   :\AgdaSymbol{ ∀}\AgdaBound{\{}\AgdaSymbol{Γ\}}\AgdaBound{(}A :\AgdaDatatype{ T}y \AgdaSymbol{Γ)}\AgdaBound{(}B :\AgdaDatatype{ T}y \AgdaSymbol{Γ}) →\AgdaDatatype{ T}y \AgdaBound{(}Γ , \AgdaSymbol{B})\AgdaFunction{
\_+tm}\_  :\AgdaSymbol{ ∀}\AgdaBound{\{}Γ \AgdaSymbol{A\}}\AgdaBound{(}a :\AgdaDatatype{ T}m \AgdaSymbol{A)}\AgdaBound{(}B :\AgdaDatatype{ T}y \AgdaSymbol{Γ}) →\AgdaDatatype{ T}m \AgdaBound{(}A\AgdaFunction{ +}T \AgdaSymbol{B})   \AgdaFunction{
\_+S}\_   :\AgdaSymbol{ ∀}\AgdaBound{\{}Γ \AgdaSymbol{Δ\}}\AgdaBound{(}δ : Γ ⇒ \AgdaSymbol{Δ)}\AgdaBound{(}B :\AgdaDatatype{ T}y \AgdaSymbol{Γ}) → \AgdaBound{(}Γ , \AgdaSymbol{B}) ⇒ Δ   
\<%
\end{code}


\AgdaHide{
\begin{code}%
\>\AgdaComment{
-- \_+T\_   : \{Γ : Con\}            (A : Ty Γ)   → (B : Ty Γ) → Ty (Γ , B)  } \AgdaComment{
-- \_+tm\_  : \{Γ : Con\}\{A : Ty Γ\}  (a : Tm A)   → (B : Ty Γ) → Tm (A +T B)  } \AgdaComment{
-- \_+S\_   : \{Γ : Con\}\{Δ : Con\}   (δ : Γ ⇒ Δ)  → (B : Ty Γ) → (Γ , B) ⇒ Δ  } \<%
\end{code}
}

%We could first define the weakening rule and substitution for types.

\AgdaHide{
\begin{code}%
\>\<%
\\
\>*       \AgdaFunction{ +}T B = *\<%
\\
\>\AgdaBound{(}a\AgdaInductiveConstructor{ =}h \AgdaSymbol{b})\AgdaFunction{ +}T B = a\AgdaFunction{ +t}m B\AgdaInductiveConstructor{ =}h b\AgdaFunction{ +t}m B

\<%
\\
\>*        [ δ\AgdaFunction{ ]}T = * \<%
\\
\>\AgdaBound{(}a\AgdaInductiveConstructor{ =}h \AgdaSymbol{b}) [ δ\AgdaFunction{ ]}T = a [ δ\AgdaFunction{ ]t}m\AgdaInductiveConstructor{ =}h b [ δ\AgdaFunction{ ]t}m

\<%
\end{code}
}
To define variables we have to use the weakening rules. We
use typed de Bruijn indices to define variables as either the rightmost
variable of the context, or some variable in the context which can be
found by cancelling the rightmost variable along with each $\AgdaInductiveConstructor{vS}$. The
coherence constants are one of the major part of this syntax, which
are primitive terms of the primitive types in contractible contexts
which will be introduced later. Since contexts, types, variables and
terms are all mutually defined, most of their properties have to
be proved simultaneously.


\begin{code}%
\>\AgdaKeyword{
dat}a\AgdaDatatype{ Va}r\AgdaKeyword{ wher}e
 \AgdaInductiveConstructor{ v}0 :\AgdaSymbol{ ∀}\AgdaBound{\{}\AgdaSymbol{Γ\}}\AgdaBound{\{}A :\AgdaDatatype{ T}y \AgdaSymbol{Γ}\}              →\AgdaDatatype{ Va}r \AgdaBound{(}A\AgdaFunction{ +}T \AgdaSymbol{A})
 \AgdaInductiveConstructor{ v}S :\AgdaSymbol{ ∀}\AgdaBound{\{}\AgdaSymbol{Γ\}}\AgdaBound{\{}A B :\AgdaDatatype{ T}y \AgdaSymbol{Γ\}}\AgdaBound{(}x :\AgdaDatatype{ Va}r \AgdaSymbol{A}) →\AgdaDatatype{ Va}r \AgdaBound{(}A\AgdaFunction{ +}T \AgdaSymbol{B})
\<%
\end{code}
A term can be either a variable or a coherence constant ($\AgdaInductiveConstructor{coh}$).
It encodes all constants for arbitrary types in a contractible context. 

\begin{code}%
\>\AgdaKeyword{
dat}a\AgdaDatatype{ T}m\AgdaKeyword{ wher}e
 \AgdaInductiveConstructor{ va}r  :\AgdaSymbol{ ∀}\AgdaBound{\{}\AgdaSymbol{Γ\}}\AgdaBound{\{}A :\AgdaDatatype{ T}y \AgdaSymbol{Γ}\} →\AgdaDatatype{ Va}r A →\AgdaDatatype{ T}m A
 \AgdaInductiveConstructor{ co}h  :\AgdaSymbol{ ∀}\AgdaBound{\{}Γ \AgdaSymbol{Δ}\} →\AgdaDatatype{ isCont}r Δ → \AgdaBound{(}δ : Γ ⇒ \AgdaSymbol{Δ}) 
       → \AgdaBound{(}A :\AgdaDatatype{ T}y \AgdaSymbol{Δ}) →\AgdaDatatype{ T}m \AgdaBound{(}A [ δ\AgdaFunction{ ]}\AgdaSymbol{T})
\<%
\end{code}

\AgdaHide{
\begin{code}%
\>\AgdaComment{
\{-
-- the symbol is \textbackslash||


data TyU : Set
data VarU : Set
data TmU : Set


∥\_∥Ty : \{Γ : Con\} → Ty Γ → TyU
∥\_∥V : \{Γ : Con\}\{A : Ty Γ\} → Var A → VarU
∥\_∥Tm : \{Γ : Con\}\{A : Ty Γ\} → Tm A → TmU

data TyU where
  *     : TyU
  \_=h\_  : \{A : TyU\} → (a b : TmU) → TyU

data VarU where
  v0 : VarU
  vS : VarU → VarU

data TmU where
  var : VarU → TmU
  coh : TyU → TmU


∥ * ∥Ty = *
∥ \_=h\_ \{A\} a b ∥Ty =  \_=h\_ \{ ∥ A ∥Ty \} ∥ a ∥Tm ∥ b ∥Tm

∥\_∥Ty-inj : \{Γ : Con\} → (a b : Ty Γ) → ∥ a ∥Ty ≡ ∥ b ∥Ty → a ≡ b
∥\_∥Ty-inj * * refl = refl
∥\_∥Ty-inj * (a =h b) ()
∥\_∥Ty-inj (a =h b) * ()
∥\_∥Ty-inj (\_=h\_ \{A\} a b) (\_=h\_ \{A₁\} a₁ b₁) eq = \{!eq!\}


∥ v0 ∥V = v0
∥ vS a ∥V = vS ∥ a ∥V



∥ a ∥Tm = \{!!\}


data Var'' : \{Γ : Con\}(A : Ty Γ) → Set where
  v0' : \{Γ : Con\}\{A : Ty Γ\}\{B : Ty (Γ , A)\} -> (B ≡ A +T A)  → Var'' B
  vS' : \{Γ : Con\}\{A B : Ty Γ\}\{C : Ty (Γ , B)\}(x : Var'' A) → (C ≡ A +T B) → Var'' C





∥\_∥inj : \{Γ : Con\}\{A : Ty Γ\} → (a b : Var A) → ∥ a ∥ ≡ ∥ b ∥ → a ≡ b
∥\_∥inj v0 b eq = \{!b!\}
∥\_∥inj (vS a) b eq = \{!!\}
-}\}
\AgdaFunction{
cohOp}V : \AgdaBound{\{}Γ :\AgdaDatatype{ Co}\AgdaSymbol{n\}}\AgdaBound{\{}A B :\AgdaDatatype{ T}y \AgdaSymbol{Γ\}}\AgdaBound{\{}x :\AgdaDatatype{ Va}r \AgdaSymbol{A\}}\AgdaBound{(}p : A ≡ \AgdaSymbol{B}) →\AgdaInductiveConstructor{ va}r \AgdaFunction{(subs}t\AgdaDatatype{ Va}r p \AgdaSymbol{x}) ≅\AgdaInductiveConstructor{ va}r x\AgdaFunction{
cohOp}V \{x = \AgdaSymbol{x}\}\AgdaInductiveConstructor{ ref}l =\AgdaInductiveConstructor{ ref}l \AgdaInductiveConstructor{(va}r \AgdaSymbol{x})
\AgdaFunction{
cohOpV}s : \AgdaBound{\{}Γ :\AgdaDatatype{ Co}\AgdaSymbol{n\}}\AgdaBound{\{}A B C :\AgdaDatatype{ T}y \AgdaSymbol{Γ\}}\AgdaBound{\{}x :\AgdaDatatype{ Va}r \AgdaSymbol{A\}}\AgdaBound{(}p : A ≡ \AgdaSymbol{B}) →\AgdaInductiveConstructor{ va}r \AgdaInductiveConstructor{(v}S \{B = \AgdaSymbol{C}\} \AgdaFunction{(subs}t\AgdaDatatype{ Va}r p \AgdaSymbol{x)}) ≅\AgdaInductiveConstructor{ va}r \AgdaInductiveConstructor{(v}S \AgdaSymbol{x})\AgdaFunction{
cohOpV}s \{x = \AgdaSymbol{x}\}\AgdaInductiveConstructor{ ref}l =\AgdaInductiveConstructor{ ref}l \AgdaInductiveConstructor{(va}r \AgdaInductiveConstructor{(v}S \AgdaSymbol{x)})
\AgdaFunction{
coh-e}q : \AgdaBound{\{}Γ Δ :\AgdaDatatype{ Co}\AgdaSymbol{n\}}\AgdaBound{\{is}c :\AgdaDatatype{ isCont}r \AgdaSymbol{Δ\}}\AgdaBound{\{}γ δ : Γ ⇒ \AgdaSymbol{Δ\}}\AgdaBound{\{}A :\AgdaDatatype{ T}y \AgdaSymbol{Δ}\} → γ ≡ δ →\AgdaInductiveConstructor{ co}h\AgdaBound{ is}c γ A ≅\AgdaInductiveConstructor{ co}h\AgdaBound{ is}c δ A \AgdaFunction{
coh-e}q\AgdaInductiveConstructor{ ref}l =\AgdaInductiveConstructor{ ref}l \_

\<%
\end{code}
}
With variables defined, it is possible to formalise another core part of the syntactic framework, \emph{contractible
contexts}. Intuitively speaking, a context is contractible if its geometric
realization is contractible to a point. It either contains one variable of the 0-cell $*$ which is the base case, or we can extend a contractible context with a
variable of an existing type and an n-cell, namely a morphism, between the new variable and some existing variable. The graph can be drawn like branching trees.

\begin{code}%
\>\AgdaKeyword{
dat}a\AgdaDatatype{ isCont}r\AgdaKeyword{ wher}e
 \AgdaInductiveConstructor{ c}*   :\AgdaDatatype{ isCont}r \AgdaInductiveConstructor{(}ε , \AgdaSymbol{*})
 \AgdaInductiveConstructor{ ex}t  :\AgdaSymbol{ ∀}\AgdaBound{\{}\AgdaSymbol{Γ}\} →\AgdaDatatype{ isCont}r Γ → \AgdaBound{\{}A :\AgdaDatatype{ T}y \AgdaSymbol{Γ\}}\AgdaBound{(}x :\AgdaDatatype{ Va}r \AgdaSymbol{A}) 
       →\AgdaDatatype{ isCont}r \AgdaBound{(}Γ , A , \AgdaInductiveConstructor{(va}r \AgdaInductiveConstructor{(v}S \AgdaSymbol{x})\AgdaInductiveConstructor{ =}h\AgdaInductiveConstructor{ va}r\AgdaInductiveConstructor{ v}\AgdaSymbol{0)})     
\<%
\end{code}
Context morphisms are defined inductively similarly to contexts. A context morphism is a list of terms corresponding to the list of types in the context on the right hand side of the morphism.

\begin{code}%
\>\AgdaKeyword{
dat}a\AgdaDatatype{ \_⇒}\_\AgdaKeyword{ wher}e
  •    :\AgdaSymbol{ ∀}\AgdaBound{\{}\AgdaSymbol{Γ}\} → Γ ⇒ ε
 \AgdaInductiveConstructor{ \_,}\_  :\AgdaSymbol{ ∀}\AgdaBound{\{}Γ \AgdaSymbol{Δ\}}\AgdaBound{(}δ : Γ ⇒ \AgdaSymbol{Δ)}\AgdaBound{\{}A :\AgdaDatatype{ T}y \AgdaSymbol{Δ\}}\AgdaBound{(}a :\AgdaDatatype{ T}m \AgdaBound{(}A [ δ\AgdaFunction{ ]}\AgdaSymbol{T)})
       → Γ ⇒ \AgdaBound{(}Δ , \AgdaSymbol{A})
\<%
\end{code}

\AgdaHide{
\begin{code}%
\>\AgdaFunction{
hom}≡ : \AgdaBound{\{}Γ :\AgdaDatatype{ Co}\AgdaSymbol{n\}}\AgdaBound{\{}A\AgdaBound{ A}' :\AgdaDatatype{ T}y \AgdaSymbol{Γ}\}
                \AgdaBound{\{}a :\AgdaDatatype{ T}m \AgdaSymbol{A\}}\AgdaBound{\{a}' :\AgdaDatatype{ T}m\AgdaBound{ A}\AgdaSymbol{'\}}\AgdaBound{(}q : a ≅\AgdaBound{ a}\AgdaSymbol{'})
                \AgdaBound{\{}b :\AgdaDatatype{ T}m \AgdaSymbol{A\}}\AgdaBound{\{b}' :\AgdaDatatype{ T}m\AgdaBound{ A}\AgdaSymbol{'\}}\AgdaBound{(}r : b ≅\AgdaBound{ b}\AgdaSymbol{'})
                → \AgdaBound{(}a\AgdaInductiveConstructor{ =}h \AgdaSymbol{b}) ≡ \AgdaBound{(a}'\AgdaInductiveConstructor{ =}h\AgdaBound{ b}\AgdaSymbol{'})\AgdaFunction{
hom}≡ \AgdaBound{\{}\AgdaSymbol{Γ}\} \AgdaSymbol{\{}\AgdaBound{.A}\AgdaSymbol{'}\} \AgdaBound{\{A}\AgdaSymbol{'}\} \AgdaSymbol{\{}\AgdaBound{.a}\AgdaSymbol{'}\} \AgdaBound{\{a}\AgdaSymbol{'}\} \AgdaInductiveConstructor{(ref}l \AgdaBound{.a}\AgdaSymbol{'}) \AgdaSymbol{\{}\AgdaBound{.b}\AgdaSymbol{'}\} \AgdaBound{\{b}\AgdaSymbol{'}\} \AgdaInductiveConstructor{(ref}l \AgdaBound{.b}\AgdaSymbol{'}) =\AgdaInductiveConstructor{ ref}l

\AgdaFunction{
cm-e}q : \AgdaBound{\{}Γ Δ :\AgdaDatatype{ Co}\AgdaSymbol{n\}}\AgdaBound{\{}γ δ : Γ ⇒ \AgdaSymbol{Δ\}}\AgdaBound{\{}A :\AgdaDatatype{ T}y \AgdaSymbol{Δ}\}
        \AgdaBound{\{}a :\AgdaDatatype{ T}m \AgdaBound{(}A [ γ\AgdaFunction{ ]}\AgdaSymbol{T)\}}\AgdaBound{\{a}' :\AgdaDatatype{ T}m \AgdaBound{(}A [ δ\AgdaFunction{ ]}\AgdaSymbol{T)}\} 
        → γ ≡ δ → a ≅\AgdaBound{ a}' 
        →\AgdaDatatype{ \_≡}\_\AgdaSymbol{ \{\_}\} \AgdaBound{\{}Γ ⇒ \AgdaBound{(}Δ , \AgdaSymbol{A)}\} \AgdaBound{(}γ , \AgdaSymbol{a}) \AgdaBound{(}δ ,\AgdaBound{ a}\AgdaSymbol{'})\AgdaFunction{
cm-e}q\AgdaInductiveConstructor{ ref}l \AgdaInductiveConstructor{(ref}l\AgdaSymbol{ \_}) =\AgdaInductiveConstructor{ ref}l

\<%
\end{code}
}


\subsection{Lemmas}

The following lemmas are essential for constructions and theorem
proving later.  The first set of lemmas states that to substitute a
type, a variable, a term, or a context morphism with two context
morphisms consecutively, is equivalent to substitute with the
composition of the two context morphisms:

\begin{code}%
\>\AgdaFunction{
[⊚]}T    :\AgdaSymbol{ ∀}\AgdaBound{\{}Γ Δ Θ \AgdaSymbol{A\}}\AgdaBound{\{}θ : Δ ⇒ \AgdaSymbol{Θ\}}\AgdaBound{\{}δ : Γ ⇒ \AgdaSymbol{Δ}\} 
        → A [ θ ⊚ δ\AgdaFunction{ ]}T ≡ \AgdaBound{(}A [ θ\AgdaFunction{ ]}\AgdaSymbol{T}\AgdaFunction{)}[ δ\AgdaFunction{ ]}T  
\AgdaFunction{
[⊚]}v    :\AgdaSymbol{ ∀}\AgdaBound{\{}Γ Δ Θ \AgdaSymbol{A\}}\AgdaBound{(}x :\AgdaDatatype{ Va}r \AgdaSymbol{A)}\AgdaBound{\{}θ : Δ ⇒ \AgdaSymbol{Θ\}}\AgdaBound{\{}δ : Γ ⇒ \AgdaSymbol{Δ}\}
        → x [ θ ⊚ δ\AgdaFunction{ ]}V ≅ \AgdaBound{(}x [ θ\AgdaFunction{ ]}\AgdaSymbol{V}) [ δ\AgdaFunction{ ]t}m
\AgdaFunction{
[⊚]t}m   :\AgdaSymbol{ ∀}\AgdaBound{\{}Γ Δ Θ \AgdaSymbol{A\}}\AgdaBound{(}a :\AgdaDatatype{ T}m \AgdaSymbol{A)}\AgdaBound{\{}θ : Δ ⇒ \AgdaSymbol{Θ\}}\AgdaBound{\{}δ : Γ ⇒ \AgdaSymbol{Δ}\}
        → a [ θ ⊚ δ\AgdaFunction{ ]t}m ≅ \AgdaBound{(}a [ θ\AgdaFunction{ ]t}\AgdaSymbol{m}) [ δ\AgdaFunction{ ]t}m
\AgdaFunction{
⊚asso}c  :\AgdaSymbol{ ∀}\AgdaBound{\{}Γ Δ Θ \AgdaSymbol{Ω\}}\AgdaBound{(}γ : Θ ⇒ \AgdaSymbol{Ω)}\AgdaBound{\{}θ : Δ ⇒ \AgdaSymbol{Θ\}}\AgdaBound{\{}δ : Γ ⇒ \AgdaSymbol{Δ}\}  
        → \AgdaBound{(}γ ⊚ \AgdaSymbol{θ}) ⊚ δ ≡ γ ⊚ \AgdaBound{(}θ ⊚ \AgdaSymbol{δ})  
\<%
\end{code}



\AgdaHide{
\begin{code}%
\>\<%
\\
\>•       ⊚ δ = •\<%
\\
\>\AgdaBound{(}δ , \AgdaSymbol{a}) ⊚\AgdaBound{ δ}' = \AgdaBound{(}δ ⊚\AgdaBound{ δ}\AgdaSymbol{'}) , a [\AgdaBound{ δ}'\AgdaFunction{ ]t}m ⟦\AgdaFunction{ [⊚]}T ⟫

\<%
\end{code}
}

The second set states that weakening inside substitution is equivalent to weakening outside:

\begin{code}%
\>\AgdaFunction{
[+S]}T   :\AgdaSymbol{ ∀}\AgdaBound{\{}Γ Δ A \AgdaSymbol{B\}}\AgdaBound{\{}δ : Γ ⇒ \AgdaSymbol{Δ}\}
        → A [ δ\AgdaFunction{ +}S B\AgdaFunction{ ]}T ≡ \AgdaBound{(}A [ δ\AgdaFunction{ ]}\AgdaSymbol{T})\AgdaFunction{ +}T B 
\AgdaFunction{
[+S]t}m  :\AgdaSymbol{ ∀}\AgdaBound{\{}Γ Δ A \AgdaSymbol{B\}}\AgdaBound{(}a :\AgdaDatatype{ T}m \AgdaSymbol{A)}\AgdaBound{\{}δ : Γ ⇒ \AgdaSymbol{Δ}\}
        → a [ δ\AgdaFunction{ +}S B\AgdaFunction{ ]t}m ≅ \AgdaBound{(}a [ δ\AgdaFunction{ ]t}\AgdaSymbol{m})\AgdaFunction{ +t}m B
\AgdaFunction{
[+S]}S   :\AgdaSymbol{ ∀}\AgdaBound{\{}Γ Δ Θ \AgdaSymbol{B\}}\AgdaBound{\{}δ : Δ ⇒ \AgdaSymbol{Θ\}}\AgdaBound{\{}γ : Γ ⇒ \AgdaSymbol{Δ}\}
        → δ ⊚ \AgdaBound{(}γ\AgdaFunction{ +}S \AgdaSymbol{B}) ≡ \AgdaBound{(}δ ⊚ \AgdaSymbol{γ})\AgdaFunction{ +}S B
\<%
\end{code}
%There are also some auxiliary functions derived from these lemmas. For instance, the function shown below is used a lot in proofs.
\AgdaHide{
\begin{code}%
\>\AgdaFunction{
wk-tm}+      : \AgdaBound{\{}Γ Δ :\AgdaDatatype{ Co}\AgdaSymbol{n\}}\AgdaBound{\{}A :\AgdaDatatype{ T}y \AgdaSymbol{Δ\}}\AgdaBound{\{}δ : Γ ⇒ \AgdaSymbol{Δ\}}\AgdaBound{(}B :\AgdaDatatype{ T}y \AgdaSymbol{Γ}) 
            →\AgdaDatatype{ T}m \AgdaBound{(}A [ δ\AgdaFunction{ ]}T\AgdaFunction{ +}T \AgdaSymbol{B}) →\AgdaDatatype{ T}m \AgdaBound{(}A [ δ\AgdaFunction{ +}S B\AgdaFunction{ ]}\AgdaSymbol{T})\AgdaFunction{
wk-tm}+ B t  = t ⟦\AgdaFunction{ [+S]}T ⟫
\<%
\end{code}
}
\AgdaHide{
\begin{code}%
\>\<%
\\
\>•      \AgdaFunction{ +}S B = •\<%
\\
\>\AgdaBound{(}δ , \AgdaSymbol{a})\AgdaFunction{ +}S B = \AgdaBound{(}δ\AgdaFunction{ +}S \AgdaSymbol{B}) ,\AgdaFunction{ wk-tm}+ B \AgdaBound{(}a\AgdaFunction{ +t}m \AgdaSymbol{B})

\AgdaFunction{
[+S]}T \{A = \AgdaSymbol{*}\}     =\AgdaInductiveConstructor{ ref}l\AgdaFunction{
[+S]}T \{A = a\AgdaInductiveConstructor{ =}h \AgdaSymbol{b}\} =\AgdaFunction{ hom}≡ \AgdaFunction{([+S]t}m \AgdaSymbol{a}) \AgdaFunction{([+S]t}m \AgdaSymbol{b})
\<%
\end{code}
}
We can cancel the last term in the substitution for weakened objects
since weakening doesn't introduce new variables in types and terms.

\begin{code}%
\>\AgdaFunction{
+T[,]}T    :\AgdaSymbol{ ∀}\AgdaBound{\{}Γ Δ A \AgdaSymbol{B\}}\AgdaBound{\{}δ : Γ ⇒ \AgdaSymbol{Δ\}}\AgdaBound{\{}b :\AgdaDatatype{ T}m \AgdaBound{(}B [ δ\AgdaFunction{ ]}\AgdaSymbol{T)}\} 
          → \AgdaBound{(}A\AgdaFunction{ +}T \AgdaSymbol{B}) [ δ , b\AgdaFunction{ ]}T ≡ A [ δ\AgdaFunction{ ]}T
\AgdaFunction{
+tm[,]t}m  :\AgdaSymbol{ ∀}\AgdaBound{\{}Γ Δ A \AgdaSymbol{B\}}\AgdaBound{\{}δ : Γ ⇒ \AgdaSymbol{Δ\}}\AgdaBound{\{}c :\AgdaDatatype{ T}m \AgdaBound{(}B [ δ\AgdaFunction{ ]}\AgdaSymbol{T)}\}
          → \AgdaBound{(}a :\AgdaDatatype{ T}m \AgdaSymbol{A}) 
          → \AgdaBound{(}a\AgdaFunction{ +t}m \AgdaSymbol{B}) [ δ , c\AgdaFunction{ ]t}m ≅ a [ δ\AgdaFunction{ ]t}m 
\<%
\end{code}
\AgdaHide{
\begin{code}%
\>\<%
\\
\>\AgdaInductiveConstructor{(va}r \AgdaSymbol{x})    \AgdaFunction{ +t}m B =\AgdaInductiveConstructor{ va}r \AgdaInductiveConstructor{(v}S \AgdaSymbol{x})\<%
\\
\>\AgdaInductiveConstructor{(co}h\AgdaBound{ c}Δ δ \AgdaSymbol{A})\AgdaFunction{ +t}m B =\AgdaInductiveConstructor{ co}h\AgdaBound{ c}Δ \AgdaBound{(}δ\AgdaFunction{ +}S \AgdaSymbol{B}) A ⟦\AgdaFunction{ sy}m\AgdaFunction{ [+S]}T ⟫ 
\AgdaFunction{
cong+t}m : \AgdaBound{\{}Γ :\AgdaDatatype{ Co}\AgdaSymbol{n\}}\AgdaBound{\{}A B C :\AgdaDatatype{ T}y \AgdaSymbol{Γ\}}\AgdaBound{\{}a :\AgdaDatatype{ T}m \AgdaSymbol{A\}}\AgdaBound{\{}b :\AgdaDatatype{ T}m \AgdaSymbol{B}\} → 
          a ≅ b
        → a\AgdaFunction{ +t}m C ≅ b\AgdaFunction{ +t}m C\AgdaFunction{
cong+t}m \AgdaInductiveConstructor{(ref}l\AgdaSymbol{ \_}) =\AgdaInductiveConstructor{ ref}l \_
\AgdaFunction{
cong+tm}2 : \AgdaBound{\{}Γ :\AgdaDatatype{ Co}\AgdaSymbol{n\}}\AgdaBound{\{}A B C :\AgdaDatatype{ T}y \AgdaSymbol{Γ}\}
           \AgdaBound{\{}a :\AgdaDatatype{ T}m \AgdaSymbol{B\}}\AgdaBound{(}p : A ≡ \AgdaSymbol{B}) 
         → a\AgdaFunction{ +t}m C ≅ a ⟦ p ⟫\AgdaFunction{ +t}m C\AgdaFunction{
cong+tm}2\AgdaInductiveConstructor{ ref}l =\AgdaInductiveConstructor{ ref}l \_

\AgdaFunction{
wk-}T : \AgdaBound{\{}Δ :\AgdaDatatype{ Co}\AgdaSymbol{n}\}
       \AgdaBound{\{}A B C :\AgdaDatatype{ T}y \AgdaSymbol{Δ}\}
       → A ≡ B → A\AgdaFunction{ +}T C ≡ B\AgdaFunction{ +}T C\AgdaFunction{
wk-}T\AgdaInductiveConstructor{ ref}l =\AgdaInductiveConstructor{ ref}l
\AgdaFunction{
wk-t}m : \AgdaBound{\{}Γ Δ :\AgdaDatatype{ Co}\AgdaSymbol{n}\}
         \AgdaBound{\{}A :\AgdaDatatype{ T}y \AgdaSymbol{Δ\}}\AgdaBound{\{}δ : Γ ⇒ \AgdaSymbol{Δ}\}
         \AgdaBound{\{}B :\AgdaDatatype{ T}y \AgdaSymbol{Δ\}}\AgdaBound{\{}b :\AgdaDatatype{ T}m \AgdaBound{(}B [ δ\AgdaFunction{ ]}\AgdaSymbol{T)}\}  
         →\AgdaDatatype{ T}m \AgdaBound{(}A [ δ\AgdaFunction{ ]}\AgdaSymbol{T}) →\AgdaDatatype{ T}m\AgdaSymbol{ (}\AgdaBound{(}A\AgdaFunction{ +}T \AgdaSymbol{B}) [ δ , b\AgdaFunction{ ]}\AgdaSymbol{T})\AgdaFunction{
wk-t}m t = t ⟦\AgdaFunction{ +T[,]}T ⟫
\AgdaInductiveConstructor{
v}0   [ δ , a\AgdaFunction{ ]}V =\AgdaFunction{ wk-t}m a\AgdaInductiveConstructor{
v}S x [ δ , a\AgdaFunction{ ]}V =\AgdaFunction{ wk-t}m \AgdaBound{(}x [ δ\AgdaFunction{ ]}\AgdaSymbol{V})

\AgdaFunction{
wk-co}h : \AgdaBound{\{}Γ Δ :\AgdaDatatype{ Co}\AgdaSymbol{n}\}
         \AgdaBound{\{}A :\AgdaDatatype{ T}y \AgdaSymbol{Δ\}}\AgdaBound{\{}δ : Γ ⇒ \AgdaSymbol{Δ}\}
         \AgdaBound{\{}B :\AgdaDatatype{ T}y \AgdaSymbol{Δ\}}\AgdaBound{\{}b :\AgdaDatatype{ T}m \AgdaBound{(}B [ δ\AgdaFunction{ ]}\AgdaSymbol{T)}\}  
         \AgdaBound{\{}t :\AgdaDatatype{ T}m \AgdaBound{(}A [ δ\AgdaFunction{ ]}\AgdaSymbol{T)}\} 
         →\AgdaFunction{ wk-t}m \{B = \AgdaSymbol{B}\} \{b = \AgdaSymbol{b}\} t ≅ t\AgdaFunction{
wk-co}h =\AgdaFunction{ cohO}p\AgdaFunction{ +T[,]}T
\AgdaFunction{
wk-coh}+ : \AgdaBound{\{}Γ Δ :\AgdaDatatype{ Co}\AgdaSymbol{n}\}
         \AgdaBound{\{}A :\AgdaDatatype{ T}y \AgdaSymbol{Δ\}}\AgdaBound{\{}δ : Γ ⇒ \AgdaSymbol{Δ}\}
         \AgdaBound{\{}B :\AgdaDatatype{ T}y \AgdaSymbol{Γ}\} 
         \AgdaBound{\{}x :\AgdaDatatype{ T}m \AgdaBound{(}A [ δ\AgdaFunction{ ]}T\AgdaFunction{ +}T \AgdaSymbol{B)}\}
          →\AgdaFunction{ wk-tm}+ B x ≅ x\AgdaFunction{
wk-coh}+ =\AgdaFunction{ cohO}p\AgdaFunction{ [+S]}T
\AgdaFunction{
wk-ho}m : \AgdaBound{\{}Γ Δ :\AgdaDatatype{ Co}\AgdaSymbol{n}\}
         \AgdaBound{\{}A :\AgdaDatatype{ T}y \AgdaSymbol{Δ\}}\AgdaBound{\{}δ : Γ ⇒ \AgdaSymbol{Δ}\}
         \AgdaBound{\{}B :\AgdaDatatype{ T}y \AgdaSymbol{Δ\}}\AgdaBound{\{}b :\AgdaDatatype{ T}m \AgdaBound{(}B [ δ\AgdaFunction{ ]}\AgdaSymbol{T)}\}  
         \AgdaBound{\{}x y :\AgdaDatatype{ T}m \AgdaBound{(}A [ δ\AgdaFunction{ ]}\AgdaSymbol{T)}\}
         → \AgdaFunction{(wk-t}m \{B = \AgdaSymbol{B}\} \{b = \AgdaSymbol{b}\} x\AgdaInductiveConstructor{ =}h\AgdaFunction{ wk-t}m \{B = \AgdaSymbol{B}\} \{b = \AgdaSymbol{b}\} \AgdaSymbol{y}) ≡ \AgdaBound{(}x\AgdaInductiveConstructor{ =}h \AgdaSymbol{y})\AgdaFunction{
wk-ho}m =\AgdaFunction{ hom}≡\AgdaFunction{ wk-co}h\AgdaFunction{ wk-co}h

\AgdaFunction{
wk-hom}+ : \AgdaBound{\{}Γ Δ :\AgdaDatatype{ Co}\AgdaSymbol{n}\}
         \AgdaBound{\{}A :\AgdaDatatype{ T}y \AgdaSymbol{Δ\}}\AgdaBound{\{}δ : Γ ⇒ \AgdaSymbol{Δ}\}
         \AgdaBound{\{}B :\AgdaDatatype{ T}y \AgdaSymbol{Γ}\} 
         \AgdaBound{\{}x y :\AgdaDatatype{ T}m \AgdaBound{(}A [ δ\AgdaFunction{ ]}T\AgdaFunction{ +}T \AgdaSymbol{B)}\}
         → \AgdaFunction{(wk-tm}+ B x\AgdaInductiveConstructor{ =}h\AgdaFunction{ wk-tm}+ B \AgdaSymbol{y}) ≡ \AgdaBound{(}x\AgdaInductiveConstructor{ =}h \AgdaSymbol{y})\AgdaFunction{
wk-hom}+ =\AgdaFunction{ hom}≡\AgdaFunction{ wk-coh}+\AgdaFunction{ wk-coh}+

\AgdaFunction{
wk-}⊚ : \AgdaBound{\{}Γ Δ Θ :\AgdaDatatype{ Co}\AgdaSymbol{n}\}
       \AgdaBound{\{}θ : Δ ⇒ \AgdaSymbol{Θ\}}\AgdaBound{\{}δ : Γ ⇒ \AgdaSymbol{Δ\}}\AgdaBound{\{}A :\AgdaDatatype{ T}y \AgdaSymbol{Θ}\}
       →\AgdaDatatype{ T}m\AgdaSymbol{ (}\AgdaBound{(}A [ θ\AgdaFunction{ ]}\AgdaSymbol{T}\AgdaFunction{)}[ δ\AgdaFunction{ ]}\AgdaSymbol{T}) →\AgdaDatatype{ T}m \AgdaBound{(}A [ θ ⊚ δ\AgdaFunction{ ]}\AgdaSymbol{T})\AgdaFunction{
wk-}⊚ t = t ⟦\AgdaFunction{ [⊚]}T ⟫
\AgdaFunction{
[+S]}S \{δ = \AgdaSymbol{•}\} =\AgdaInductiveConstructor{ ref}l\AgdaFunction{
[+S]}S \{δ = δ , \AgdaSymbol{a}\} =\AgdaFunction{ cm-e}q\AgdaFunction{ [+S]}S \AgdaFunction{(cohO}p\AgdaFunction{ [⊚]}T ∾ \AgdaFunction{([+S]t}m a ∾\AgdaFunction{ cong+tm}2\AgdaFunction{ [⊚]}\AgdaSymbol{T}) ∾\AgdaFunction{ wk-coh}+\AgdaFunction{ -}\AgdaSymbol{¹})

\AgdaFunction{
wk+S+}T :\AgdaSymbol{ ∀}\AgdaBound{\{}Γ Δ :\AgdaDatatype{ Co}\AgdaSymbol{n\}}\AgdaBound{\{}A :\AgdaDatatype{ T}y \AgdaSymbol{Γ\}}\AgdaBound{\{}B :\AgdaDatatype{ T}y \AgdaSymbol{Δ}\}
          \AgdaBound{\{}\AgdaSymbol{γ\}}\AgdaBound{\{}\AgdaSymbol{C}\} → 
          A [ γ\AgdaFunction{ ]}T ≡ C 
       → A [ γ\AgdaFunction{ +}S B\AgdaFunction{ ]}T ≡ C\AgdaFunction{ +}T B\AgdaFunction{
wk+S+}T\AgdaBound{ e}q =\AgdaFunction{ tran}s\AgdaFunction{ [+S]}T \AgdaFunction{(wk-}T\AgdaBound{ e}\AgdaSymbol{q})
\AgdaFunction{
wk+S+t}m : \AgdaBound{\{}Γ Δ :\AgdaDatatype{ Co}\AgdaSymbol{n\}}\AgdaBound{\{}A :\AgdaDatatype{ T}y \AgdaSymbol{Γ\}}\AgdaBound{\{}B :\AgdaDatatype{ T}y \AgdaSymbol{Δ}\}
          \AgdaBound{(}a :\AgdaDatatype{ T}m \AgdaSymbol{A)}\AgdaBound{\{}C :\AgdaDatatype{ T}y \AgdaSymbol{Δ\}}\AgdaBound{\{}γ : Δ ⇒ \AgdaSymbol{Γ\}}\AgdaBound{\{}c :\AgdaDatatype{ T}m \AgdaSymbol{C}\} →
          a [ γ\AgdaFunction{ ]t}m ≅ c 
        → a [ γ\AgdaFunction{ +}S B\AgdaFunction{ ]t}m ≅ c\AgdaFunction{ +t}m B\AgdaFunction{
wk+S+t}m \_\AgdaBound{ e}q =\AgdaFunction{ [+S]t}m \_ ∾\AgdaFunction{ cong+t}m\AgdaBound{ e}q

\AgdaFunction{
wk+S+}S :\AgdaSymbol{ ∀}\AgdaBound{\{}Γ Δ\AgdaBound{ Δ}₁ :\AgdaDatatype{ Co}\AgdaSymbol{n\}}\AgdaBound{\{}δ : Δ ⇒\AgdaBound{ Δ}\AgdaSymbol{₁\}}\AgdaBound{\{}γ : Γ ⇒ \AgdaSymbol{Δ\}}\AgdaBound{\{}ω : Γ ⇒\AgdaBound{ Δ}\AgdaSymbol{₁\}}\AgdaBound{\{}B :\AgdaDatatype{ T}y \AgdaSymbol{Γ}\}
       → δ ⊚ γ ≡ ω
       → δ ⊚ \AgdaBound{(}γ\AgdaFunction{ +}S \AgdaSymbol{B}) ≡ ω\AgdaFunction{ +}S B\AgdaFunction{
wk+S+}S\AgdaBound{ e}q =\AgdaFunction{ tran}s\AgdaFunction{ [+S]}S \AgdaFunction{(con}g\AgdaSymbol{ (}λ x → x\AgdaFunction{ +}S\AgdaSymbol{ \_})\AgdaBound{ e}\AgdaSymbol{q})

\AgdaFunction{
[⊚]}T \{A = \AgdaSymbol{*}\} =\AgdaInductiveConstructor{ ref}l\AgdaFunction{
[⊚]}T \{A =\AgdaInductiveConstructor{ \_=h}\_ \AgdaBound{\{}\AgdaSymbol{A}\} a \AgdaSymbol{b}\} =\AgdaFunction{ hom}≡ \AgdaFunction{([⊚]t}m\AgdaSymbol{ \_}) \AgdaFunction{([⊚]t}m\AgdaSymbol{ \_}) 
\AgdaFunction{
+T[,]}T \{A = \AgdaSymbol{*}\} =\AgdaInductiveConstructor{ ref}l\AgdaFunction{
+T[,]}T \{A =\AgdaInductiveConstructor{ \_=h}\_ \AgdaBound{\{}\AgdaSymbol{A}\} a \AgdaSymbol{b}\} =\AgdaFunction{ hom}≡  \AgdaFunction{(+tm[,]t}m\AgdaSymbol{ \_}) \AgdaFunction{(+tm[,]t}m\AgdaSymbol{ \_})

\<%
\end{code}
}
Most of the substitutions are defined as usual, except the one for coherence constants. We do
substitution in the context morphism part of the coherence constants.

\begin{code}%
\>\AgdaInductiveConstructor{
va}r x       [ δ\AgdaFunction{ ]t}m = x [ δ\AgdaFunction{ ]}V\AgdaInductiveConstructor{
co}h\AgdaBound{ c}Δ γ A  [ δ\AgdaFunction{ ]t}m =\AgdaInductiveConstructor{ co}h\AgdaBound{ c}Δ \AgdaBound{(}γ ⊚ \AgdaSymbol{δ}) A ⟦\AgdaFunction{ sy}m\AgdaFunction{ [⊚]}T ⟫
\<%
\end{code}


\AgdaHide{
\begin{code}%
\>\AgdaComment{
-- congruenc}e
\AgdaFunction{
cong}T : ∀ \AgdaBound{\{}Γ Δ :\AgdaDatatype{ Co}\AgdaSymbol{n\}}\AgdaBound{\{}A B :\AgdaDatatype{ T}y \AgdaSymbol{Δ\}}\AgdaBound{\{}γ : Γ ⇒ \AgdaSymbol{Δ}\} → A ≡ B → A [ γ\AgdaFunction{ ]}T ≡ B [ γ\AgdaFunction{ ]}T \AgdaFunction{
cong}T\AgdaInductiveConstructor{ ref}l =\AgdaInductiveConstructor{ ref}l

\AgdaFunction{
congT}2 : ∀ \AgdaBound{\{}Γ \AgdaSymbol{Δ}\} → \AgdaBound{\{}δ γ : Δ ⇒ \AgdaSymbol{Γ\}}\AgdaBound{\{}A :\AgdaDatatype{ T}y \AgdaSymbol{Γ}\} → δ ≡ γ → A [ δ\AgdaFunction{ ]}T ≡ A [ γ\AgdaFunction{ ]}T\AgdaFunction{
congT}2\AgdaInductiveConstructor{ ref}l =\AgdaInductiveConstructor{ ref}l 
\AgdaFunction{
cong}V : \AgdaBound{\{}Γ Δ :\AgdaDatatype{ Co}\AgdaSymbol{n\}}\AgdaBound{\{}A B :\AgdaDatatype{ T}y \AgdaSymbol{Δ\}}\AgdaBound{\{}a :\AgdaDatatype{ Va}r \AgdaSymbol{A\}}\AgdaBound{\{}b :\AgdaDatatype{ Va}r \AgdaSymbol{B}\} →
    \AgdaInductiveConstructor{ va}r a ≅\AgdaInductiveConstructor{ va}r b → 
     \AgdaBound{\{}δ : Γ ⇒ \AgdaSymbol{Δ}\} 
     → a [ δ\AgdaFunction{ ]}V ≅ b [ δ\AgdaFunction{ ]}V\AgdaFunction{
cong}V \AgdaBound{\{}\AgdaSymbol{Γ}\} \AgdaBound{\{}\AgdaSymbol{Δ}\} \AgdaSymbol{\{}\AgdaBound{.}\AgdaSymbol{B}\} \AgdaBound{\{}\AgdaSymbol{B}\} \AgdaSymbol{\{}\AgdaBound{.}\AgdaSymbol{b}\} \AgdaBound{\{}\AgdaSymbol{b}\} \AgdaInductiveConstructor{(ref}l\AgdaSymbol{ .}\AgdaInductiveConstructor{(va}r \AgdaSymbol{b}\AgdaSymbol{)}) =\AgdaInductiveConstructor{ ref}l \_
\AgdaFunction{
congt}m : \AgdaBound{\{}Γ Δ :\AgdaDatatype{ Co}\AgdaSymbol{n\}}\AgdaBound{\{}A B :\AgdaDatatype{ T}y \AgdaSymbol{Γ\}}\AgdaBound{\{}a :\AgdaDatatype{ T}m \AgdaSymbol{A\}}\AgdaBound{\{}b :\AgdaDatatype{ T}m \AgdaSymbol{B}\}
      \AgdaBound{(}p : a ≅ \AgdaSymbol{b}) → 
      \AgdaBound{\{}δ : Δ ⇒ \AgdaSymbol{Γ}\}
      → a [ δ\AgdaFunction{ ]t}m ≅ b [ δ\AgdaFunction{ ]t}m\AgdaFunction{
congt}m \AgdaInductiveConstructor{(ref}l\AgdaSymbol{ \_}) =\AgdaInductiveConstructor{ ref}l \_ 
\AgdaFunction{
congtm}2 : \AgdaBound{\{}Γ Δ :\AgdaDatatype{ Co}\AgdaSymbol{n\}}\AgdaBound{\{}A :\AgdaDatatype{ T}y \AgdaSymbol{Γ\}}\AgdaBound{\{}a :\AgdaDatatype{ T}m \AgdaSymbol{A}\}
          \AgdaBound{\{}δ γ : Δ ⇒ \AgdaSymbol{Γ}\} →
          \AgdaBound{(}p : δ ≡ \AgdaSymbol{γ})
        → a [ δ\AgdaFunction{ ]t}m ≅ a [ γ\AgdaFunction{ ]t}m\AgdaFunction{
congtm}2\AgdaInductiveConstructor{ ref}l =\AgdaInductiveConstructor{ ref}l \_
\AgdaFunction{
⊚asso}c • =\AgdaInductiveConstructor{ ref}l\AgdaFunction{
⊚asso}c \AgdaInductiveConstructor{(\_,}\_ γ \AgdaBound{\{}\AgdaSymbol{A}\} \AgdaSymbol{a}) =\AgdaFunction{ cm-e}q \AgdaFunction{(⊚asso}c \AgdaSymbol{γ}) 
    \AgdaFunction{(cohO}p\AgdaFunction{ [⊚]}T 
    ∾ \AgdaFunction{(congt}m \AgdaFunction{(cohO}p\AgdaFunction{ [⊚]}\AgdaSymbol{T})
    ∾\AgdaSymbol{ (}\AgdaFunction{(cohO}p\AgdaFunction{ [⊚]}T 
    ∾\AgdaFunction{ [⊚]t}m \AgdaSymbol{a})\AgdaFunction{ -}\AgdaSymbol{¹))})

\AgdaFunction{
[⊚]}v \AgdaInductiveConstructor{(v}0 \AgdaBound{\{Γ}\AgdaSymbol{₁}\} \AgdaBound{\{}\AgdaSymbol{A\}}) \AgdaBound{\{}θ , \AgdaSymbol{a}\}  =\AgdaFunction{ wk-co}h ∾\AgdaFunction{ cohO}p\AgdaFunction{ [⊚]}T ∾\AgdaFunction{ congt}m \AgdaFunction{(cohO}p\AgdaFunction{ +T[,]}T\AgdaFunction{ -}\AgdaSymbol{¹}) \AgdaFunction{
[⊚]}v \AgdaInductiveConstructor{(v}S \AgdaBound{\{Γ}\AgdaSymbol{₁}\} \AgdaBound{\{}\AgdaSymbol{A}\} \AgdaBound{\{}\AgdaSymbol{B}\} \AgdaSymbol{x}) \AgdaBound{\{}θ , \AgdaSymbol{a}\} = 
 \AgdaFunction{ wk-co}h ∾ \AgdaFunction{([⊚]}v x ∾ \AgdaFunction{(congt}m \AgdaFunction{(cohO}p\AgdaFunction{ +T[,]}\AgdaSymbol{T})\AgdaFunction{ -}\AgdaSymbol{¹)})


\AgdaFunction{
[⊚]t}m \AgdaInductiveConstructor{(va}r \AgdaSymbol{x}) =\AgdaFunction{ [⊚]}v x\AgdaFunction{
[⊚]t}m \AgdaInductiveConstructor{(co}h c γ \AgdaSymbol{A}) =\AgdaFunction{ cohO}p \AgdaFunction{(sy}m\AgdaFunction{ [⊚]}\AgdaSymbol{T}) ∾ \AgdaFunction{(coh-e}q \AgdaFunction{(sy}m \AgdaFunction{(⊚asso}c \AgdaSymbol{γ)}) ∾\AgdaFunction{ cohO}p \AgdaFunction{(sy}m\AgdaFunction{ [⊚]}\AgdaSymbol{T})\AgdaFunction{ -}\AgdaSymbol{¹}) ∾\AgdaFunction{ congt}m \AgdaFunction{(cohO}p \AgdaFunction{(sy}m\AgdaFunction{ [⊚]}\AgdaSymbol{T})\AgdaFunction{ -}\AgdaSymbol{¹})

\AgdaFunction{
⊚w}k :\AgdaSymbol{ ∀}\AgdaBound{\{}Γ Δ\AgdaBound{ Δ}\AgdaSymbol{₁\}}\AgdaBound{\{}B :\AgdaDatatype{ T}y \AgdaSymbol{Δ\}}\AgdaBound{(}γ : Δ ⇒\AgdaBound{ Δ}\AgdaSymbol{₁)}\AgdaBound{\{}δ : Γ ⇒ \AgdaSymbol{Δ\}}\AgdaBound{\{}c :\AgdaDatatype{ T}m \AgdaBound{(}B [ δ\AgdaFunction{ ]}\AgdaSymbol{T)}\} → \AgdaBound{(}γ\AgdaFunction{ +}S \AgdaSymbol{B}) ⊚ \AgdaBound{(}δ , \AgdaSymbol{c}) ≡ γ ⊚ δ\AgdaFunction{
⊚w}k • =\AgdaInductiveConstructor{ ref}l\AgdaFunction{
⊚w}k \AgdaInductiveConstructor{(\_,}\_ γ \AgdaBound{\{}\AgdaSymbol{A}\} \AgdaSymbol{a}) =\AgdaFunction{ cm-e}q \AgdaFunction{(⊚w}k \AgdaSymbol{γ}) \AgdaFunction{(cohO}p\AgdaFunction{ [⊚]}T ∾ \AgdaFunction{(congt}m \AgdaFunction{(cohO}p\AgdaFunction{ [+S]}\AgdaSymbol{T}) ∾\AgdaFunction{ +tm[,]t}m \AgdaSymbol{a}) ∾\AgdaFunction{ cohO}p\AgdaFunction{ [⊚]}T\AgdaFunction{ -}\AgdaSymbol{¹})
\AgdaFunction{
+tm[,]t}m \AgdaInductiveConstructor{(va}r \AgdaSymbol{x}) =\AgdaFunction{ cohO}p\AgdaFunction{ +T[,]}T\AgdaFunction{
+tm[,]t}m \AgdaInductiveConstructor{(co}h x γ \AgdaSymbol{A}) =\AgdaFunction{ congt}m \AgdaFunction{(cohO}p \AgdaFunction{(sy}m\AgdaFunction{ [+S]}\AgdaSymbol{T)}) ∾\AgdaFunction{ cohO}p \AgdaFunction{(sy}m\AgdaFunction{ [⊚]}\AgdaSymbol{T}) ∾\AgdaFunction{ coh-e}q \AgdaFunction{(⊚w}k \AgdaSymbol{γ}) ∾\AgdaFunction{ cohO}p \AgdaFunction{(sy}m\AgdaFunction{ [⊚]}\AgdaSymbol{T})\AgdaFunction{ -}¹


\AgdaFunction{
[+S]}V : \AgdaBound{\{}Γ Δ :\AgdaDatatype{ Co}\AgdaSymbol{n\}}\AgdaBound{\{}A :\AgdaDatatype{ T}y \AgdaSymbol{Δ}\}
         \AgdaBound{(}x :\AgdaDatatype{ Va}r \AgdaSymbol{A)}\AgdaBound{\{}δ : Γ ⇒ \AgdaSymbol{Δ}\}
         \AgdaBound{\{}B :\AgdaDatatype{ T}y \AgdaSymbol{Γ}\}
         → x [ δ\AgdaFunction{ +}S B\AgdaFunction{ ]}V ≅ \AgdaBound{(}x [ δ\AgdaFunction{ ]}\AgdaSymbol{V})\AgdaFunction{ +t}m B\AgdaFunction{
[+S]}V\AgdaInductiveConstructor{ v}0 \AgdaInductiveConstructor{\{\_,}\_ δ \AgdaBound{\{}\AgdaSymbol{A}\} \AgdaSymbol{a}\} =\AgdaFunction{ wk-co}h ∾\AgdaFunction{ wk-coh}+ ∾\AgdaFunction{ cong+tm}2\AgdaFunction{ +T[,]}T\AgdaFunction{
[+S]}V \AgdaInductiveConstructor{(v}S \AgdaSymbol{x}) \AgdaBound{\{}δ , \AgdaSymbol{a}\} =\AgdaFunction{ wk-co}h ∾\AgdaFunction{ [+S]}V x ∾\AgdaFunction{ cong+tm}2\AgdaFunction{ +T[,]}T

\AgdaFunction{
[+S]t}m \AgdaInductiveConstructor{(va}r \AgdaSymbol{x}) =\AgdaFunction{ [+S]}V x\AgdaFunction{
[+S]t}m \AgdaInductiveConstructor{(co}h x δ \AgdaSymbol{A}) =\AgdaFunction{ cohO}p \AgdaFunction{(sy}m\AgdaFunction{ [⊚]}\AgdaSymbol{T}) ∾\AgdaFunction{ coh-e}q\AgdaFunction{ [+S]}S ∾\AgdaFunction{ cohO}p \AgdaFunction{(sy}m\AgdaFunction{ [+S]}\AgdaSymbol{T})\AgdaFunction{ -}¹ ∾\AgdaFunction{ cong+tm}2 \AgdaFunction{(sy}m\AgdaFunction{ [⊚]}\AgdaSymbol{T})

\AgdaComment{
-- some widely-used context}s
\AgdaFunction{
x:}* :\AgdaDatatype{ Co}n\AgdaFunction{
x:}* = ε , *
\AgdaFunction{
x:*,y:*,α:x=}y :\AgdaDatatype{ Co}n\AgdaFunction{
x:*,y:*,α:x=}y =\AgdaFunction{ x:}* , * , \AgdaInductiveConstructor{(va}r \AgdaInductiveConstructor{(v}S\AgdaInductiveConstructor{ v}\AgdaSymbol{0})\AgdaInductiveConstructor{ =}h\AgdaInductiveConstructor{ va}r\AgdaInductiveConstructor{ v}\AgdaSymbol{0})
\AgdaFunction{
v}X :\AgdaDatatype{ T}m \AgdaFunction{\{x:*,y:*,α:x=}\AgdaSymbol{y}\} *\AgdaFunction{
v}X =\AgdaInductiveConstructor{ va}r \AgdaInductiveConstructor{(v}S \AgdaInductiveConstructor{(v}S\AgdaInductiveConstructor{ v}\AgdaSymbol{0)})
\AgdaFunction{
v}Y :\AgdaDatatype{ T}m \AgdaFunction{\{x:*,y:*,α:x=}\AgdaSymbol{y}\} *\AgdaFunction{
v}Y =\AgdaInductiveConstructor{ va}r \AgdaInductiveConstructor{(v}S\AgdaInductiveConstructor{ v}\AgdaSymbol{0})
\AgdaFunction{
v}α :\AgdaDatatype{ T}m \AgdaFunction{\{x:*,y:*,α:x=}\AgdaSymbol{y}\} \AgdaFunction{(v}X\AgdaInductiveConstructor{ =}h\AgdaFunction{ v}\AgdaSymbol{Y})\AgdaFunction{
v}α =\AgdaInductiveConstructor{ va}r\AgdaInductiveConstructor{ v}0
\AgdaFunction{
x:*,y:*,α:x=y,z:*,β:y=}z :\AgdaDatatype{ Co}n\AgdaFunction{
x:*,y:*,α:x=y,z:*,β:y=}z =\AgdaFunction{ x:*,y:*,α:x=}y , * , \AgdaInductiveConstructor{(va}r \AgdaInductiveConstructor{(v}S \AgdaInductiveConstructor{(v}S\AgdaInductiveConstructor{ v}\AgdaSymbol{0)})\AgdaInductiveConstructor{ =}h\AgdaInductiveConstructor{ va}r\AgdaInductiveConstructor{ v}\AgdaSymbol{0})
\AgdaFunction{
v}Z :\AgdaDatatype{ T}m \AgdaFunction{\{x:*,y:*,α:x=y,z:*,β:y=}\AgdaSymbol{z}\} *\AgdaFunction{
v}Z =\AgdaInductiveConstructor{ va}r \AgdaInductiveConstructor{(v}S\AgdaInductiveConstructor{ v}\AgdaSymbol{0})
\AgdaFunction{
v}β :\AgdaDatatype{ T}m \AgdaFunction{\{x:*,y:*,α:x=y,z:*,β:y=}\AgdaSymbol{z}\} \AgdaFunction{(v}Y\AgdaFunction{ +t}m \_\AgdaFunction{ +t}m \_\AgdaInductiveConstructor{ =}h\AgdaFunction{ v}\AgdaSymbol{Z})\AgdaFunction{
v}β =\AgdaInductiveConstructor{ va}r\AgdaInductiveConstructor{ v}0











\AgdaComment{
\{-
data Var' : \{Γ : Con\}(A : Ty Γ) → Set where
  v0 : \{Γ : Con\}\{A : Ty Γ\} → Var' \{Γ , A\} (A +T A)
  vS : \{Γ : Con\}\{A B : Ty Γ\}\{C : Ty (Γ , A)\}(x : Var' (B +T A)) → Var' (B +T A +T C)

open import Data.Empty

var-ne : ∀ (A : Ty ε) → Var \{ε\} A → ⊥
var-ne A ()

+T-unif : ∀(Γ : Con)(A B C : Ty Γ) → 
          A +T B ≡ C +T B → A ≡ C
+T-unif Γ * B * refl = refl
+T-unif Γ * B (a =h b) ()
+T-unif Γ (a =h b) B * ()
+T-unif Γ (a =h b) B (a₁ =h b₁) eq = \{!!\}

v0only : ∀ (A : Ty ε) → (x : Var \{ε , A\} (A +T A)) → x ≡ v0
v0only A x = \{!x!\}


\_≟v\_ : ∀(Γ : Con)(A : Ty Γ)(a b : Var A) → Dec (a ≡ b)
\_≟v\_ .(ε , A) .(A +T A) (v0 \{ε\} \{A\}) b = \{!b!\}
\_≟v\_ .(Γ , A , A₁) .(A₁ +T A₁) (v0 \{Γ , A\} \{A₁\}) b = \{!!\}
\_≟v\_ .(Γ , B) .(A +T B) (vS \{Γ\} \{A\} \{B\} a) b = \{!!\}




var x ≟tm var x₁ = \{!!\}
var x₁ ≟tm coh x δ A = no (λ ())
coh x δ A ≟tm b = \{!b!\}

-}\}

\<%
\end{code}
}

\section{Some Important Derivable Constructions}

\input{IdentityContextMorphisms}

\input{Suspension}

\input{GroupoidStructure}

\input{Telescopes2}

\section{Semantics}

\subsection{Globular Types}

\input{GlobularTypes}

%\txa{Can we show that substitution is correct}
%\txa{Some discussion on why we don't need coherence laws.}

\input{Semantics}



\section{Conclusion}

In this paper, we present an implementation of \wog{} following  Brunerie's work. Briefly speaking, we define the syntax of the type theory \tig{}, then a weak $\omega$-groupoid is a globular set with the interpretation of the syntax. To overcome some technical problems, we use heterogeneous equality for terms, some auxiliary functions and loop context in all implementation. We construct the identity morphisms and verify some groupoid laws in the syntactic framework. The suspensions for all sorts of objects are also defined for other later constructions.

There is still a lot of work to do within the syntactic framework. For instance, we would like to investigate the relation between the \tig{} and a Type Theory with equality types and J eliminator which is called $\mathcal{T}_{eq}$. One direction is to simulate the J eliminator syntactically in \tig{} as we mentioned before, the other direction is to derive J using $coh$ if we can prove that the $\mathcal{T}_{eq}$ is a weak $\omega$-groupoid. The syntax could be simplified by adopting categories with families. An alternative may be to use higher inductive types directly to formalize the syntax of type theory. 

We would like to formalise a proof of that  $\AgdaFunction{Idω}$ is a weak $\omega$-groupoid, but the base set in a globular set is an h-set which is incompatible with $\AgdaFunction{Idω}$. Perhaps we could solve the problem by instead proving a syntactic result, namely that the theory we have presented here and the theory of equality types with J are equivalence. Finally, to model the Type Theory with \wog{} and to eliminate the univalence axiom would be the most challenging task in the future. 

\bibliography{latex/my.bib}

\end{document}
